more robust testing and minor bug fixes

grackle_test.go
@@ -21,13 +21,27 @@ func TestGetCoqOutput(t *testing.T) {
 func TestCalendarExample(t *testing.T) {
 	grackleBuffer := bytes.NewBuffer(make([]byte, 0, 10000))
 	grackleOutput := bufio.NewWriter(grackleBuffer)
-	protoFiles := "testdata/proto"
-	gooseOutput := "example"
-	coqLogicalPath := "Grackle.example"
-	coqPhysicalPath := "example"
-	goOutputPath := "example"
-	goPackage := "github.com/mjschwenne/grackle/example"
+	protoFiles := "testdata/proto/calendar"
+	gooseOutput := "testdata/out/goose"
+	coqLogicalPath := "Grackle.test"
+	coqPhysicalPath := "testdata/out/coq"
+	goOutputPath := "testdata/out/go"
+	goPackage := "github.com/mjschwenne/grackle/testdata/out/go"
 	Grackle(&protoFiles, &gooseOutput, &coqLogicalPath, &coqPhysicalPath, &goOutputPath, &goPackage, grackleOutput)
 	grackleOutput.Flush()
 	golden.Assert(t, grackleBuffer.String(), "golden/calendar.golden")
+}
+
+func TestCompleteExample(t *testing.T) {
+	grackleBuffer := bytes.NewBuffer(make([]byte, 0, 10000))
+	grackleOutput := bufio.NewWriter(grackleBuffer)
+	protoFiles := "testdata/proto/complete/"
+	gooseOutput := "testdata/out/goose"
+	coqLogicalPath := "Grackle.test"
+	coqPhysicalPath := "testdata/out/coq"
+	goOutputPath := "testdata/out/go"
+	goPackage := "github.com/mjschwenne/grackle/testdata/out/go"
+	Grackle(&protoFiles, &gooseOutput, &coqLogicalPath, &coqPhysicalPath, &goOutputPath, &goPackage, grackleOutput)
+	grackleOutput.Flush()
+	golden.Assert(t, grackleBuffer.String(), "golden/complete.golden")
 }
