testdata/out/go/completeint_gk/completeint_gk.go
@@ -1,0 +1,45 @@
+package completeint_gk
+
+import (
+	"github.com/tchajed/marshal"
+)
+
+type S struct {
+	One   uint32
+	Two   uint32
+	Three uint32
+	Four  uint64
+	Five  uint64
+	Six   uint64
+}
+
+func (c *S) approxSize() uint64 {
+	return 0
+}
+
+func Marshal(c *S, prefix []byte) []byte {
+	var enc = prefix
+
+	enc = marshal.WriteInt32(enc, c.One)
+	enc = marshal.WriteInt32(enc, c.Two)
+	enc = marshal.WriteInt32(enc, c.Three)
+	enc = marshal.WriteInt(enc, c.Four)
+	enc = marshal.WriteInt(enc, c.Five)
+	enc = marshal.WriteInt(enc, c.Six)
+
+	return enc
+}
+
+func Unmarshal(s []byte) (*S, []byte) {
+	c := new(S)
+	var enc = s // Needed for goose compatibility
+
+	c.One, enc = marshal.ReadInt32(enc)
+	c.Two, enc = marshal.ReadInt32(enc)
+	c.Three, enc = marshal.ReadInt32(enc)
+	c.Four, enc = marshal.ReadInt(enc)
+	c.Five, enc = marshal.ReadInt(enc)
+	c.Six, enc = marshal.ReadInt(enc)
+
+	return c, enc
+}
