testdata/out/go/completemessage_gk/completemessage_gk.go
@@ -1,0 +1,38 @@
+package completemessage_gk
+
+import (
+	"github.com/goose-lang/primitive"
+
+	"github.com/mjschwenne/grackle/testdata/out/go/completeint_gk"
+	"github.com/mjschwenne/grackle/testdata/out/go/completeslice_gk"
+)
+
+type S struct {
+	Int *completeint_gk.S
+	Slc *completeslice_gk.S
+}
+
+func (c *S) approxSize() uint64 {
+	return 0
+}
+
+func Marshal(c *S, prefix []byte) []byte {
+	var enc = prefix
+
+	primitive.Assume(c.Int != nil)
+	enc = completeint_gk.Marshal(c.Int, enc)
+	primitive.Assume(c.Slc != nil)
+	enc = completeslice_gk.Marshal(c.Slc, enc)
+
+	return enc
+}
+
+func Unmarshal(s []byte) (*S, []byte) {
+	c := new(S)
+	var enc = s // Needed for goose compatibility
+
+	c.Int, enc = completeint_gk.Unmarshal(enc)
+	c.Slc, enc = completeslice_gk.Unmarshal(enc)
+
+	return c, enc
+}
