testdata/out/go/completeslice_gk/completeslice_gk.go
@@ -1,0 +1,44 @@
+package completeslice_gk
+
+import (
+	"github.com/tchajed/marshal"
+)
+
+type S struct {
+	Strg string
+	Byte []byte
+}
+
+func (c *S) approxSize() uint64 {
+	return 0
+}
+
+func Marshal(c *S, prefix []byte) []byte {
+	var enc = prefix
+
+	strgBytes := []byte(c.Strg)
+	enc = marshal.WriteInt(enc, uint64(len(strgBytes)))
+	enc = marshal.WriteBytes(enc, strgBytes)
+	enc = marshal.WriteInt(enc, uint64(len(c.Byte)))
+	enc = marshal.WriteBytes(enc, c.Byte)
+
+	return enc
+}
+
+func Unmarshal(s []byte) (*S, []byte) {
+	c := new(S)
+	var enc = s // Needed for goose compatibility
+
+	var strgLen uint64
+	var strgBytes []byte
+	strgLen, enc = marshal.ReadInt(enc)
+	strgBytes, enc = marshal.ReadBytesCopy(enc, strgLen)
+	c.Strg = string(strgBytes)
+	var byteLen uint64
+	var byteBytes []byte
+	byteLen, enc = marshal.ReadInt(enc)
+	byteBytes, enc = marshal.ReadBytesCopy(enc, byteLen)
+	c.Byte = byteBytes
+
+	return c, enc
+}
