testdata/out/goose/github_com/mjschwenne/grackle/testdata/out/go/event_gk.v
@@ -42,7 +42,7 @@ Definition Unmarshal: val :=
     let: ("0_ret", "1_ret") := marshal.ReadInt (![slice.T byteT] "enc") in
     "nameLen" <-[uint64T] "0_ret";;
     "enc" <-[slice.T byteT] "1_ret";;
-    let: ("0_ret", "1_ret") := marshal.ReadBytes (![slice.T byteT] "enc") (![uint64T] "nameLen") in
+    let: ("0_ret", "1_ret") := marshal.ReadBytesCopy (![slice.T byteT] "enc") (![uint64T] "nameLen") in
     "nameBytes" <-[slice.T byteT] "0_ret";;
     "enc" <-[slice.T byteT] "1_ret";;
     struct.storeF S "Name" "e" (StringFromBytes (![slice.T byteT] "nameBytes"));;
