testdata/out/coq/completeint_proof.v
@@ -1,0 +1,124 @@
+From Perennial.program_proof Require Import grove_prelude.
+From Perennial.program_proof Require Import marshal_stateless_proof.
+From Goose Require Import github_com.mjschwenne.grackle.testdata.out.go.completeint_gk.
+
+Module completeInt.
+Section completeInt.
+
+Typeclasses Opaque app.
+
+Context `{!heapGS Σ}.
+
+Record C :=
+    mkC {
+        one : u32;
+        two : u32;
+        three : u32;
+        four : u64;
+        five : u64;
+        six : u64;
+        }.
+
+Definition has_encoding (encoded:list u8) (args:C) : Prop :=
+  encoded = (u32_le args.(one)) ++
+              (u32_le args.(two)) ++
+              (u32_le args.(three)) ++
+              (u64_le args.(four)) ++
+              (u64_le args.(five)) ++
+              (u64_le args.(six)).
+
+Definition own (args_ptr: loc) (args: C) (dq: dfrac) : iProp Σ :=
+  "Hargs_one" ∷ args_ptr ↦[completeint_gk.S :: "One"]{dq} #args.(one) ∗
+  "Hargs_two" ∷ args_ptr ↦[completeint_gk.S :: "Two"]{dq} #args.(two) ∗
+  "Hargs_three" ∷ args_ptr ↦[completeint_gk.S :: "Three"]{dq} #args.(three) ∗
+  "Hargs_four" ∷ args_ptr ↦[completeint_gk.S :: "Four"]{dq} #args.(four) ∗
+  "Hargs_five" ∷ args_ptr ↦[completeint_gk.S :: "Five"]{dq} #args.(five) ∗
+  "Hargs_six" ∷ args_ptr ↦[completeint_gk.S :: "Six"]{dq} #args.(six).
+
+Lemma wp_Encode (args_ptr:loc) (args:C) (pre_sl:Slice.t) (prefix:list u8) (dq: dfrac):
+  {{{
+        own args_ptr args dq ∗
+        own_slice pre_sl byteT (DfracOwn 1) prefix
+  }}}
+    completeint_gk.Marshal #args_ptr (slice_val pre_sl)
+  {{{
+        enc enc_sl, RET (slice_val enc_sl);
+        ⌜has_encoding enc args⌝ ∗
+        own args_ptr args dq ∗
+        own_slice enc_sl byteT (DfracOwn 1) (prefix ++ enc)
+  }}}.
+
+Proof.
+  iIntros (?) "H HΦ". iDestruct "H" as "[Hown Hsl]". iNamed "Hown".
+  wp_rec. wp_pures.
+  wp_apply (wp_ref_to); first by val_ty.
+  iIntros (?) "Hptr". wp_pures.
+
+  wp_loadField. wp_load. wp_apply (wp_WriteInt32 with "[$Hsl]").
+  iIntros (?) "Hsl". wp_store.
+
+  wp_loadField. wp_load. wp_apply (wp_WriteInt32 with "[$Hsl]").
+  iIntros (?) "Hsl". wp_store.
+
+  wp_loadField. wp_load. wp_apply (wp_WriteInt32 with "[$Hsl]").
+  iIntros (?) "Hsl". wp_store.
+  wp_loadField. wp_load. wp_apply (wp_WriteInt with "[$Hsl]").
+  iIntros (?) "Hsl". wp_store.
+  wp_loadField. wp_load. wp_apply (wp_WriteInt with "[$Hsl]").
+  iIntros (?) "Hsl". wp_store.
+  wp_loadField. wp_load. wp_apply (wp_WriteInt with "[$Hsl]").
+  iIntros (?) "Hsl". wp_store.
+
+
+  wp_load. iApply "HΦ". iModIntro. rewrite -?app_assoc.
+  iFrame. iPureIntro.
+
+  done.
+Qed.
+
+Lemma wp_Decode enc enc_sl (args: C) (suffix: list u8) (dq: dfrac):
+  {{{
+        ⌜has_encoding enc args⌝ ∗
+        own_slice_small enc_sl byteT dq (enc ++ suffix)
+  }}}
+    completeint_gk.Unmarshal (slice_val enc_sl)
+  {{{
+        args_ptr suff_sl, RET (#args_ptr, suff_sl); own args_ptr args (DfracOwn 1) ∗
+                                                    own_slice_small suff_sl byteT dq suffix
+  }}}.
+
+Proof.
+  iIntros (?) "[%Henc Hsl] HΦ". wp_rec.
+  wp_apply wp_allocStruct; first by val_ty.
+  iIntros (?) "Hstruct". wp_pures.
+  wp_apply wp_ref_to; first done.
+  iIntros (?) "Hptr". wp_pures.
+  iDestruct (struct_fields_split with "Hstruct") as "HH".
+  iNamed "HH".
+
+  rewrite Henc. rewrite -?app_assoc.
+
+  wp_load. wp_apply (wp_ReadInt32 with "[$Hsl]"). iIntros (?) "Hsl".
+  wp_pures. wp_storeField. wp_store.
+
+  wp_load. wp_apply (wp_ReadInt32 with "[$Hsl]"). iIntros (?) "Hsl".
+  wp_pures. wp_storeField. wp_store.
+
+  wp_load. wp_apply (wp_ReadInt32 with "[$Hsl]"). iIntros (?) "Hsl".
+  wp_pures. wp_storeField. wp_store.
+
+  wp_load. wp_apply (wp_ReadInt with "[$Hsl]"). iIntros (?) "Hsl".
+  wp_pures. wp_storeField. wp_store.
+
+  wp_load. wp_apply (wp_ReadInt with "[$Hsl]"). iIntros (?) "Hsl".
+  wp_pures. wp_storeField. wp_store.
+
+  wp_load. wp_apply (wp_ReadInt with "[$Hsl]"). iIntros (?) "Hsl".
+  wp_pures. wp_storeField. wp_store.
+
+  wp_load. wp_pures. iApply "HΦ". iModIntro. rewrite ?string_to_bytes_to_string. iFrame.
+Qed.
+
+End completeInt.
+End completeInt.
+
