Makefile
@@ -1,4 +1,4 @@
-SRC_DIRS := 'perennial' 'example'
+SRC_DIRS := 'perennial' 'example' 'testdata/out'
 ALL_VFILES := $(shell find $(SRC_DIRS) \
 							-not -path "perennial/external/coqutil/etc/coq-scripts/*" \
 						    -not -path "perennial/new*/*" \
