build_go.fish
@@ -1,8 +1,0 @@
-#!/usr/bin/env fish 
-
-go build $argv
-if test $status = 0
-    echo "Compliation Successful"
-else
-    echo "Compliation Unsuccessful"
-end
