run_tests.fish
@@ -1,0 +1,14 @@
+#!/usr/bin/env fish
+
+echo "Cleaning old tests..."
+rm -rf testdata/out/*
+echo "Running grackle..."
+go run ./cmd/grackle/ -coq-logical-path Grackle.test -coq-physical-path testdata/out/coq/ -go-output-path testdata/out/go -go-package github.com/mjschwenne/grackle/testdata/out/go -goose-output testdata/out/goose/ testdata/proto/calendar
+go run ./cmd/grackle/ -coq-logical-path Grackle.test -coq-physical-path testdata/out/coq/ -go-output-path testdata/out/go -go-package github.com/mjschwenne/grackle/testdata/out/go -goose-output testdata/out/goose/ testdata/proto/complete
+echo "Checking grackle go..."
+go build (find ./testdata/out/go/ -mindepth 1 -maxdepth 1 -type d)
+echo "Checking grackle coq..."
+rm .coqdeps.d
+make -j(nproc) -s (find testdata/out/coq -name "*.v" | sed -e "s/\.v\$/\.vo/g")
+echo "Running grackle tests..."
+go test .
